src/bak/FunctionalSimulation.v
@@ -1,4 +1,4 @@
-Require Import Mealy.
+(* Require Import Mealy.
 Require Import Coq.Lists.List.
 
 (* Definition 2.4 (Simulation) *)
@@ -32,17 +32,15 @@ induction v.
   injection P as P P'. rewrite P. rewrite P'. trivial.
 - intros V q q' H J P. assert (K := P). apply first_letter_exi in K.
   destruct K as [r K]. destruct K as [o K]. destruct K as [K K']. destruct K' as [K' K''].
-  rewrite tra_trans_def_known in K''.
   specialize IHv with (tl V) r q'. assert (IH := H). apply IHv in IH. clear IHv.
 
   unfold funcSim in H. destruct H as [H H']. simpl.
   specialize H' with q r a o.
-  assert (G := K'').
-  
+  assert (G := K).
   apply H' in G.
   rewrite<- G.
   rewrite IH.
-  rewrite K'.
+  rewrite K''.
   simpl.
   reflexivity.
   apply J.
@@ -58,6 +56,6 @@ induction v.
   destruct C as [(qq, AQ)]. 
   destruct lemma_a_1 with M aq (a :: nil) AQ (q0 M) q.
   unfold del in J. rewrite H0 in J. injection J as J. rewrite<- J. apply H0.
-  rewrite H1. unfold del. unfold tra. rewrite K''. trivial.
-  apply K.
-Qed.
+  rewrite H1. unfold del. unfold tra. rewrite K. trivial.
+  apply K'.
+Qed. *)
